LambdaS5/coq/EjsFromJs.v
@@ -1,0 +1,136 @@
+Generalizable All Variables.
+Set Implicit Arguments.
+Require Import LjsShared.
+Require Import JsNumber.
+Require Import Utils.
+Require LjsSyntax.
+Require EjsSyntax.
+Require JsSyntax.
+Import ListNotations.
+Open Scope list_scope.
+Open Scope string_scope.
+
+Local Coercion JsNumber.of_int : Z >-> JsNumber.number.
+
+Module E := EjsSyntax.
+Module J := JsSyntax.
+
+Fixpoint js_literal_to_ejs l := 
+    match l with
+    | J.literal_null => E.expr_null
+    | J.literal_bool true => E.expr_true
+    | J.literal_bool false => E.expr_false
+    | J.literal_number n => E.expr_number n
+    | J.literal_string s => E.expr_string s
+    end.
+
+Fixpoint js_stat_block_to_ejs es :=
+    match es with
+    | nil => E.expr_undefined
+    | [e] => e
+    | e :: es' => E.expr_seq e (js_stat_block_to_ejs es')
+    end.
+
+Fixpoint js_expr_to_ejs (e : J.expr) : E.expr := 
+    let map_js_expr_to_ejs := (fix f l := match l with nil => nil | e :: l' => js_expr_to_ejs e :: f l' end) in 
+    match e with
+    | J.expr_this => E.expr_this
+    | J.expr_literal l => js_literal_to_ejs l
+    | J.expr_member e s => E.expr_get_field (js_expr_to_ejs e) (E.expr_string s) 
+    | J.expr_access e1 e2 => E.expr_get_field (js_expr_to_ejs e1) (js_expr_to_ejs e2)
+    | J.expr_unary_op o e => E.expr_op1 o (js_expr_to_ejs e) 
+    | J.expr_binary_op e1 o e2 => E.expr_op2 o (js_expr_to_ejs e1) (js_expr_to_ejs e2)
+    | J.expr_conditional e1 e2 e3 => E.expr_if (js_expr_to_ejs e1) (js_expr_to_ejs e2) (js_expr_to_ejs e3)
+    | J.expr_new e es => E.expr_new (js_expr_to_ejs e) (map_js_expr_to_ejs es)
+    | J.expr_call e es => E.expr_app (js_expr_to_ejs e) (map_js_expr_to_ejs es)
+    | _ => E.expr_undefined
+    end
+with js_stat_to_ejs (e : J.stat) : E.expr := 
+    let map_js_stat_to_ejs := (fix f l := match l with nil => nil | e :: l' => js_stat_to_ejs e :: f l' end) in
+    let js_switchclause_to_ejs c := 
+        match c with
+        | J.switchclause_intro e sts => E.case_case (js_expr_to_ejs e) (js_stat_block_to_ejs (map_js_stat_to_ejs sts))
+        end in
+    let map_js_switchclause_to_ejs := 
+        (fix f l := match l with nil => nil | e :: l' => js_switchclause_to_ejs e :: f l' end) in 
+    match e with
+    | J.stat_expr e => js_expr_to_ejs e
+    | J.stat_label s st => E.expr_label s (js_stat_to_ejs st)
+    | J.stat_block sts => js_stat_block_to_ejs (map_js_stat_to_ejs sts)
+(*    | J.stat_var_decl *)
+    | J.stat_if e st None => E.expr_if (js_expr_to_ejs e) (js_stat_to_ejs st) (E.expr_undefined)
+    | J.stat_if e st (Some st') => E.expr_if (js_expr_to_ejs e) (js_stat_to_ejs st) (js_stat_to_ejs st')
+(* TODO select implementation strategy
+    | J.stat_do_while nil st e => E.expr_label "%before" (E.expr_do_while (js_stat_to_ejs st) (js_expr_to_ejs e)) 
+*)
+    | J.stat_while nil e st => 
+        E.expr_label "%before" (E.expr_while (js_expr_to_ejs e) (js_stat_to_ejs st) E.expr_undefined)
+    | J.stat_with e st => E.expr_with (js_expr_to_ejs e) (js_stat_to_ejs st)
+    | J.stat_throw e => E.expr_throw (js_expr_to_ejs e)
+    | J.stat_return oe =>
+        let e := match oe with
+        | None => E.expr_undefined
+        | Some e => js_expr_to_ejs e
+        end in 
+        E.expr_break "%ret" e 
+    | J.stat_break lbl =>
+        let s := match lbl with
+        | J.label_empty => "%before"
+        | J.label_string s => s
+        end in 
+        E.expr_break s E.expr_undefined
+    | J.stat_continue lbl => (* TODO looks fishy! *)
+        let s := match lbl with
+        | J.label_empty => "%continue"
+        | J.label_string s => s
+        end in 
+        E.expr_break s E.expr_undefined
+    | J.stat_try st None None => js_stat_to_ejs st
+    | J.stat_try st (Some (s, st1)) None => E.expr_try_catch (js_stat_to_ejs st) s (js_stat_to_ejs st1)
+    | J.stat_try st None (Some st2) => E.expr_try_finally (js_stat_to_ejs st) (js_stat_to_ejs st2)
+    | J.stat_try st (Some (s, st1)) (Some st2) => 
+        E.expr_try_finally (E.expr_try_catch (js_stat_to_ejs st) s (js_stat_to_ejs st1)) (js_stat_to_ejs st2)
+    | J.stat_for nil oe1 oe2 oe3 st => 
+        let e1 := match oe1 with
+        | None => E.expr_undefined
+        | Some e => js_expr_to_ejs e
+        end in
+        let e2 := match oe2 with
+        | None => E.expr_undefined
+        | Some e => js_expr_to_ejs e
+        end in 
+        let e3 := match oe3 with
+        | None => E.expr_true
+        | Some e => js_expr_to_ejs e
+        end in 
+        E.expr_seq e1 (E.expr_label "%before" (E.expr_while e2 (js_stat_to_ejs st) e3))
+(* TODO decide on variable support 
+    | J.stat_for_var nil le1 oe2 oe3 st =>
+        let e2 := match oe2 with
+        | None => E.expr_undefined
+        | Some e => js_expr_to_ejs e
+        end in 
+        let e3 := match oe3 with
+        | None => E.expr_true
+        | Some e => js_expr_to_ejs e
+        end in 
+*)       
+(* TODO for-in
+    | J.stat_for_in nil lval e st => 
+        E.expr_label "%before" (E.expr_for_in s (js_expr_to_ejs e) (js_stat_to_ejs st))
+*)
+    | J.stat_switch nil e (J.switchbody_nodefault cl) => 
+        E.expr_switch (js_expr_to_ejs e) (map_js_switchclause_to_ejs cl)
+    | J.stat_switch nil e (J.switchbody_withdefault cl1 sts cl2) => 
+        E.expr_switch (js_expr_to_ejs e) 
+            (map_js_switchclause_to_ejs cl1 ++ 
+                [E.case_default (js_stat_block_to_ejs (map_js_stat_to_ejs sts))] ++ 
+                map_js_switchclause_to_ejs cl2)
+    | _ => E.expr_undefined
+    end
+with js_element_to_ejs (e : J.element) : E.expr := 
+    match e with
+    | J.element_stat st => js_stat_to_ejs st
+    | _ => E.expr_undefined
+    end
+.
